Terms are isomorphic to their de-Bruijn indexed forms

FreydSSA/Ctx.lean
@@ -159,14 +159,6 @@ theorem Ctx.EqOn.tail {ρ₁ ρ₂ : ν → ν'} {v} {Γ : Ctx ν α} (h : Ctx.E
   : Ctx.EqOn ρ₁ ρ₂ Γ
   := λ _ hx => h (hx.tail _)
 
-inductive Ctx.HasVar {ν α : Type u} (A : α) : ℕ → Ctx ν α → Prop
-  | head : Ctx.HasVar A 0 (⟨n, A⟩::Γ)
-  | tail : Ctx.HasVar A n Γ → Ctx.HasVar A (n+1) (x::Γ)
-
-structure Ctx.Ix {ν α} (Γ : Ctx ν α) (A : α) : Type where
-  val : ℕ
-  hasVar : Ctx.HasVar A val Γ
-
 structure Label (ν : Type u) (α : Type v) extends Var ν α where
   live : Ctx ν α
 
@@ -281,3 +273,142 @@ theorem Ctx.EqOn.rename {ρ₁ ρ₂ : ν → ν'} {Γ : Ctx ν α} (hΓ : Γ.Eq
 theorem Ctx.EqOn.rename_id {ρ : ν → ν} {Γ : Ctx ν α} (hΓ : Γ.EqOn ρ id)
   : Γ.rename ρ = Γ
   := hΓ.rename.trans Γ.rename_id
+
+def Ctx.deBruijn {ν α} (n : ℕ) : Ctx ν α → Ctx ℕ α
+  | [] => []
+  | ⟨_, a⟩::Γ => ⟨n, a⟩::deBruijn (n+1) Γ
+
+def Ctx.Wk.target_deBruijn {ν α} {Γ Δ : Ctx ν α} (n : ℕ) : Γ.Wk Δ → Ctx ℕ α
+  | Wk.nil => []
+  | Wk.cons x h => ⟨n, x.ty⟩::target_deBruijn (n+1) h
+  | Wk.skip _ h => target_deBruijn (n+1) h
+
+theorem Ctx.Wk.target_deBruijn_fresh {ν α} {Γ Δ : Ctx ν α} {n m : ℕ} (H: n < m)
+  : (w: Γ.Wk Δ) → Fresh n (w.target_deBruijn m)
+  | nil => Fresh.nil
+  | cons _ w => Fresh.cons (Nat.ne_of_lt H).symm (target_deBruijn_fresh (Nat.lt.step H) w)
+  | skip _ w => target_deBruijn_fresh (Nat.lt.step H) w
+
+def Ctx.Wk.deBruijn {ν α} {Γ Δ : Ctx ν α} (n : ℕ) : (w: Γ.Wk Δ)
+  → (deBruijn n Γ).Wk (w.target_deBruijn n)
+  | nil => nil
+  | cons x w => cons ⟨n, x.ty⟩ (deBruijn (n+1) w)
+  | skip hxn w => skip (w.target_deBruijn_fresh (Nat.lt.base _)) (deBruijn (n+1) w)
+
+theorem Ctx.Wk.iso_deBruijn {ν α} {Γ Δ : Ctx ν α} (n : ℕ)
+  : (w: Γ.Wk Δ) → w.Iso (w.deBruijn n)
+  | nil => Iso.nil
+  | cons _ w => Iso.cons (iso_deBruijn (n + 1) w)
+  | skip _ w => Iso.skip (iso_deBruijn (n + 1) w)
+
+inductive Ctx.HasVar {ν α : Type u} (A : α) : ℕ → ν → Ctx ν α → Prop
+  | head : Ctx.HasVar A 0 x (⟨x, A⟩::Γ)
+  | tail : x ≠ v.name → Ctx.HasVar A n x Γ → Ctx.HasVar A (n+1) x (v::Γ)
+
+structure Ctx.Ix {ν α} (Γ : Ctx ν α) (x : ν) (A : α) : Type _ where
+  val : ℕ
+  hasVar : Ctx.HasVar A val x Γ
+
+def Ctx.Ix.head {ν α} {Γ : Ctx ν α} {x : ν} {A : α} : Ctx.Ix (⟨x, A⟩::Γ) x A where
+  val := 0
+  hasVar := HasVar.head
+
+def Ctx.Ix.tail {ν α} {Γ : Ctx ν α} {v : Var ν α} {x : ν} {A : α}
+  (i : Ctx.Ix Γ x A) (h : x ≠ v.name)
+  : Ctx.Ix (v::Γ) x A where
+  val := i.val + 1
+  hasVar := HasVar.tail h i.hasVar
+
+def Ctx.Wk.var_ix {Γ : Ctx ν α} : Γ.Wk [⟨n, A⟩] → ℕ
+  | Wk.cons _ w => 0
+  | Wk.skip _ w => w.var_ix + 1
+
+theorem Ctx.var_ix_hasVar {Γ : Ctx ν α}
+  : (w: Γ.Wk [⟨x, A⟩]) → Γ.HasVar A w.var_ix x
+  | Wk.cons _ _ => Ctx.HasVar.head
+  | Wk.skip hxn w => Ctx.HasVar.tail hxn.head (var_ix_hasVar w)
+
+def Ctx.HasVar.toWk {Γ : Ctx ν α} {A : α} {n} {x} (H : Γ.HasVar A n x) : Γ.Wk [⟨x, A⟩]
+  := match n, Γ with
+  | _, [] => nomatch H
+  | 0, y::Γ =>
+    have Hxy: ⟨x, A⟩ = y := by cases H; rfl
+    Hxy ▸ Wk.cons ⟨x, A⟩ (Wk.drop Γ)
+  | n + 1, _::_ => Wk.skip
+    (match H with | tail hx _ => Fresh.cons hx Fresh.nil)
+    (toWk (by cases H; assumption))
+
+def Ctx.Wk.to_ix {Γ : Ctx ν α} {A : α} : Γ.Wk [⟨x, A⟩] → Ctx.Ix Γ x A
+  | cons _ _ => Ctx.Ix.head
+  | skip hx w => w.to_ix.tail hx.head
+
+def Ctx.Wk.to_ix' {Γ : Ctx ν α} {A : α} (w: Γ.Wk [⟨x, A⟩]) : Ctx.Ix Γ x A
+  := ⟨w.var_ix, var_ix_hasVar w⟩
+
+def Ctx.HasVar.not_empty {Γ : Ctx ν α} {A : α} {n} {x} (H : Γ.HasVar A n x) : Γ ≠ []
+  := by cases Γ with
+  | nil => cases H
+  | cons => simp
+
+def Ctx.Ix.not_empty {Γ : Ctx ν α} {x : ν} {A : α} (i : Ctx.Ix Γ x A) : Γ ≠ []
+  := i.hasVar.not_empty
+
+theorem Ctx.Wk.drop_target_deBruijn {ν α} {Γ : Ctx ν α} (n : ℕ)
+  : (w: Γ.Wk []) → w.target_deBruijn n = []
+  | Wk.nil => rfl
+  | Wk.skip _ w => drop_target_deBruijn (n+1) w
+
+--FIXME: broken
+-- theorem Ctx.Wk.var_target_deBruijn {ν α} {x: ν} {A: α} {Γ : Ctx ν α} (n : ℕ)
+--   : (w: Γ.Wk [⟨x, A⟩]) → w.target_deBruijn n = [⟨n + w.var_ix, A⟩]
+--   | cons _ w => by simp [target_deBruijn, drop_target_deBruijn, var_ix]
+--   | skip _ w =>
+--     let I := var_target_deBruijn (n + 1) w;
+--     by simp_arith [
+--       target_deBruijn, drop_target_deBruijn, var_ix, I
+--     ]
+
+--TODO: also broken...
+-- theorem Ctx.Wk.var_target_deBruijn' {ν α} {x: ν} {A: α} {Γ Δ : Ctx ν α} (n : ℕ)
+--   (w: Γ.Wk Δ) (h: Δ = [Var.mk x A]): w.target_deBruijn n = [⟨n + (h ▸ w).var_ix, A⟩]
+--   := by induction w generalizing n with
+--   | nil => cases h
+--   | cons _ w I => cases h; simp [var_ix, target_deBruijn, drop_target_deBruijn]
+--   | skip _ w I => cases h; simp_arith [var_ix, target_deBruijn, I]
+
+theorem Ctx.Wk.var_target_deBruijn' {ν α} {x : ν} {A : α} {Γ Δ : Ctx ν α} (n : ℕ)
+  (w : Γ.Wk Δ) (h : Δ = [Var.mk x A])
+  : w.target_deBruijn n = [Var.mk (n + (h ▸ w).var_ix) A]
+  := by induction w generalizing n with
+  | nil => cases h
+  | cons _ w I => cases h; simp [var_ix, target_deBruijn, drop_target_deBruijn]
+  | skip _ w I =>
+    cases h
+    simp only [target_deBruijn]
+    rw [I _ rfl]
+    simp only [var_ix]
+    rw [add_assoc, add_comm 1]
+
+theorem Ctx.Wk.var_target_deBruijn {ν α} {x : ν} {A : α} {Γ : Ctx ν α} (n : ℕ)
+  (w: Γ.Wk [⟨x, A⟩]) : w.target_deBruijn n = [⟨n + w.var_ix, A⟩]
+  := w.var_target_deBruijn' n rfl
+
+def Ctx.Wk.var_deBruijn {ν α} {Γ : Ctx ν α} {x : ν} {A : α} (n : ℕ)
+  (w : Γ.Wk [⟨x, A⟩]) : (Γ.deBruijn n).Wk [⟨n + w.var_ix, A⟩]
+  := w.var_target_deBruijn n ▸ w.deBruijn n
+
+theorem Ctx.Wk.iso_cast {ν : Type u} {α : Type v} {Γ Δ Γ' Δ' : Ctx ν α}
+  (h : Γ.Wk Δ = Γ'.Wk Δ')
+  (hΓ : Γ = Γ')
+  (hΔ : Δ = Δ')
+  (w: Γ.Wk Δ) : w.Iso (cast h w)
+  := by cases hΓ; cases hΔ; cases h; exact Iso.refl w
+
+theorem Ctx.Wk.iso_var_deBruijn {ν α} {Γ : Ctx ν α} {x : ν} {A : α} (n : ℕ)
+  (w : Γ.Wk [⟨x, A⟩]) : w.Iso (w.var_deBruijn n)
+  := Iso.trans (w.iso_deBruijn n) (by
+    simp only [var_deBruijn, Eq.rec_eq_cast]
+    apply iso_cast
+    rfl
+    apply var_target_deBruijn
+    )
